Flapjack/Tests.lean
@@ -36,6 +36,7 @@ import Flapjack.Test.CrepeSemantics
 import Flapjack.Test.Ffi
 import Flapjack.Test.LoopFfi
 import Flapjack.Test.ExactFfi
+import Flapjack.Test.CorrectnessExactFfi
 import Flapjack.Test.Stack
 import Flapjack.Test.Lab
 import Flapjack.Test.RiscVLab
